Finished HW8 P7

hw8/prob07.lean
@@ -3,15 +3,58 @@ import .src.lnat
 
 def e1 : Expr :=
   -- FILL IN HERE.
-  sorry
+  (Expr.Op Op.Add
+    (Expr.Num 1)
+    (Expr.Op Op.Add ((Expr.Op Op.Add  (Expr.Num 2)
+                                      (Expr.Num 3)))
+                    (Expr.Num 4))
+  )
+
+def e1_step : Expr :=
+  -- FILL IN HERE.
+  (Expr.Op Op.Add
+    (Expr.Num 1)
+    (Expr.Op Op.Add (Expr.Num 5) (Expr.Num 4))
+  )
+
+def e1_step_step : Expr :=
+  -- FILL IN HERE.
+  (Expr.Op Op.Add
+    (Expr.Num 1)
+    (Expr.Num  9)
+  )
 
 def e2 : Expr :=
   -- FILL IN HERE.
-  sorry
+  (Expr.Num 10)
 
 lemma evals_example :
   (val e2) ∧ (e1 ↦* e2) :=
 begin
   -- FILL IN HERE.
-  sorry
+  split,
+  {
+    apply val.VNum,
+  },
+  {
+    -- The below lines show that e1 can be stepped to e1_step
+    apply evals.CStep,
+    show Expr,
+    from e1_step,
+    apply eval.ERight,
+    apply eval.ELeft,
+    apply eval.EOp,
+    apply val.VNum,
+    apply evals.CStep,
+    show Expr,
+    from e1_step_step,
+    apply eval.ERight,
+    apply eval.EOp,
+    apply val.VNum,
+    apply evals.CStep,
+    show Expr,
+    from e2,
+    apply eval.EOp,
+    refl,
+  }
 end
